examples/Imp2Vir/Imp2Cvir.v
@@ -16,79 +16,83 @@ From Imp2Vir Require Import Imp Fin.
 
 Require Import Vec CompileExpr CvirCombinators CvirCombinatorsWF.
 
+From Vellvm Require Import SurfaceSyntax.
+Import VIR_Notations.
+
 Open Scope Z_scope.
 
 Section Imp2Cvir.
 
-Fixpoint compile (next_reg : int) (s : stmt) (env: StringMap.t int)
-: option (int * (StringMap.t int) * cvir 1 1) :=
-  match s with
-  | Skip => Some(next_reg, env, block_cvir [])
-  | Assign x e =>
+  Fixpoint compile (next_reg : int) (s : stmt) (env: StringMap.t int)
+  : option (int * (StringMap.t int) * cvir 1 1) :=
+    match s with
+    | Skip => Some(next_reg, env, block_cvir [])
+    | Assign x e =>
       '(next_reg, env, ir) <- compile_assign next_reg x e env;;
       ret (next_reg, env, block_cvir ir)
-  | Seq l r =>
+
+    | Seq l r =>
       '(next_reg, env, ir_l) <- compile next_reg l env;;
       '(next_reg, env, ir_r) <- compile next_reg r env;;
-       ret (next_reg, env, seq_cvir ir_l ir_r)
-  | While e b =>
+      ret (next_reg, env, seq_cvir ir_l ir_r)
+
+    | While e b =>
       '(cond_reg, expr_ir) <- compile_cond next_reg e env;;
       '(next_reg, _, ir) <- compile (cond_reg + 1) b env;;
       let br := branch_cvir expr_ir (texp_i1 cond_reg) in
-      let body := seq_cvir br ir in
-      let body := focus_output_cvir body (exist _ 1%nat Nat.lt_1_2) in
+      let body := merge_cvir ir (block_cvir []) : cvir 2 2 in
+      let body := seq_cvir br body in
       let ir := loop_cvir_open body in
       ret (next_reg, env, ir) : option (int * (StringMap.t int) * cvir 1 1)
-  | If e l r =>
+
+    | If e l r =>
       '(cond_reg, expr_code) <- compile_cond next_reg e env;;
       '(next_reg, _, ir_l) <- compile (cond_reg + 1) l env;;
       '(next_reg, _, ir_r) <- compile next_reg r env;;
-      let ir := branch_cvir expr_code (texp_i1 cond_reg) : cvir 1 2 in
-      let ir := seq_cvir ir ir_l : cvir 1 2 in
-      let ir := seq_cvir ir ir_r : cvir 1 2 in
+      let ir_cond := branch_cvir expr_code (texp_i1 cond_reg) : cvir 1 2 in
+      let ir_body := merge_cvir ir_l ir_r in
+      let ir := seq_cvir ir_cond ir_body in
       let ir := join_cvir ir : cvir 1 1 in
       ret (next_reg, env, ir) : option (int * (StringMap.t int) * cvir 1 1)
-  end.
+    end.
 
-(* TODO it misses cvir_inputs_used and relabel_WF properties *)
-Theorem compile_WF : forall s next_reg next_reg' env env' ir,
-compile next_reg s env = Some(next_reg', env', ir) ->
-cvir_ids_WF ir /\
-unique_bid ir.
-Proof.
-  induction s ; intros ? ? ? ? ? Heqo ; simpl in Heqo.
-  - repeat break_match ; try discriminate.
-    inversion Heqo.
-    subst.
-    split; [apply block_cvir_id_WF | apply block_cvir_unique].
-  - repeat break_match ; try discriminate.
-    inversion Heqo.
-    subst.
-    simpl in *.
-    apply IHs1 in Heqo0.
-    apply IHs2 in Heqo1.
-    split; [ apply (seq_cvir_id_WF 1 0) | apply (seq_cvir_unique 1 0)]
-    ; simpl in * ; tauto.
-  - repeat break_match ; try discriminate.
-    inversion Heqo.
-    subst.
-    simpl in *.
-    apply IHs1 in Heqo1.
-    apply IHs2 in Heqo2.
-    split; [ apply join_cvir_id_WF | apply join_cvir_unique ];
-    [> apply (seq_cvir_id_WF 1 1) | apply (seq_cvir_unique 1 1)]; try tauto;
-    (apply (seq_cvir_id_WF 1 1) + apply (seq_cvir_unique 1 1)); try tauto;
-    (apply branch_cvir_id_WF + apply branch_cvir_unique).
-  - repeat break_match ; try discriminate.
-    inversion Heqo.
-    subst.
-    apply IHs in Heqo1.
-    split; [ apply loop_cvir_open_id_WF | apply loop_cvir_open_unique ];
-    [> apply focus_output_cvir_id_WF | apply focus_output_cvir_unique ];
-    [> eapply (seq_cvir_id_WF 1 1) | eapply (seq_cvir_unique 1 1) ];
-    (apply branch_cvir_id_WF + apply branch_cvir_unique + tauto).
-  - inversion Heqo.
-    split; [ apply block_cvir_id_WF | apply block_cvir_unique ].
+  Theorem compile_WF : forall s next_reg next_reg' env env' ir,
+compile next_reg s env = Some(next_reg', env', ir) -> cvir_WF ir.
+  Proof.
+    induction s ; intros ? ? ? ? ? Heqo ; simpl in Heqo.
+    - repeat break_match ; try discriminate.
+      inversion Heqo.
+      subst. apply block_cvir_WF.
+    - repeat break_match ; try discriminate.
+      inversion Heqo.
+      subst.
+      simpl in *.
+      apply IHs1 in Heqo0.
+      apply IHs2 in Heqo1.
+      apply seq_cvir_WF ; assumption.
+    - repeat break_match ; try discriminate.
+      inversion Heqo.
+      subst.
+      simpl in *.
+      apply IHs1 in Heqo1.
+      apply IHs2 in Heqo2.
+      apply join_cvir_WF.
+      apply seq_cvir_WF.
+      apply branch_cvir_WF.
+      apply merge_cvir_WF with (ni1:= 1%nat) (no1:= 1%nat) (ir1:= c0) in Heqo2 ; assumption.
+      (* I don't understand why `apply merge_cvir_WF`` doesn't work *)
+    - repeat break_match ; try discriminate.
+      inversion Heqo.
+      subst.
+      apply IHs in Heqo1.
+      apply loop_open_cvir_WF.
+      apply seq_cvir_WF.
+      + apply branch_cvir_WF.
+      + apply merge_cvir_WF with (ni1:= 1%nat) (no1:= 1%nat)
+                                 (ni2:= 1%nat) (no2:= 1%nat)
+                                 (ir1:= c0) (ir2:= (block_cvir [])) ;
+          [ assumption | apply block_cvir_WF ].
+    - inversion Heqo. apply block_cvir_WF.
 Qed.
 
 Definition compile_imp_cvir (ir : cvir 1 1) : program :=
@@ -109,13 +113,20 @@ Definition compile_program (s : stmt) (env : StringMap.t int) :
   '(_, _, ir) <- compile 0 s env;;
   ret (compile_imp_cvir ir).
 
+
+
 Definition fact_ir := (compile_program (fact "a" "b" 5) (StringMap.empty int)).
+Definition infinite_loop_ir := (compile_program (infinite_loop) (StringMap.empty int)).
+Definition if_ir := (compile_program (trivial_if "a" "b" 0) (StringMap.empty int)).
+Definition seq_ir := (compile_program (trivial_seq "a" "b" 42) (StringMap.empty int)).
+Definition nested_if_ir := (compile_program (nested_if "a" "b" 42 43) (StringMap.empty int)).
+Definition nested_if2_ir := (compile_program (nested_if2 "a" "b" 42 43) (StringMap.empty int)).
 
-Definition if_ir :=
-  (compile_program (trivial_if "a" "b" 0) (StringMap.empty int)).
 
-Compute if_ir.
-
-Eval compute in fact_ir.
-
+(* Compute infinite_loop_ir. *)
+(* Compute seq_ir. *)
+(* Compute if_ir. *)
+(* Compute nested_if_ir. *)
+(* Compute nested_if2_ir. *)
+(* Compute fact_ir. *)
 End Imp2Cvir.
